---
title: "MLP forwards/backwards"
format: html
---

## MLP forwards/backwards mathematical derivation

This is a mathematical derivation of the MLP forward and backward propagation equations. 

(1) [Wikipedia article](https://en.wikipedia.org/wiki/Backpropagation) 
(2) [Neural Networks and Deep Learning book](http://neuralnetworksanddeeplearning.com/chap2.html).

### Forward propagation

The forward propagation can be written as:


- vectorized version
$$
\begin{flalign*}
\vec{z} &= L(\vec{x};W,\vec{b}) \quad = \vec{x} @ W  + \vec{b} \\
\vec{y} &= f(\vec{z})           \quad = tanh(\vec{z}) \\
\end{flalign*}
$$

- non-vectorized (indexed) version
$$
\begin{flalign*}
z_{j} &= L(x_i; w_{ij},b_j, \forall i) = \sum_{i} x_i \cdot w_{ij}\\
y_j &= f(z_j) = tanh(z_j) \\
\end{flalign*}
$$

- sum squared error

$$
\begin{flalign*}
e &= E(y_j; y_j^*, \forall j)= \frac{1}{2} \sum_{j} (y_j - y_j^*)^2 \\
\end{flalign*}
$$

- backpropagation

$$
\begin{flalign*}
\frac{\partial e}{\partial y_j}
&= y_j-y^*_j 
\\
\frac{\partial e}{\partial z_j}
&=
\frac{\partial e}{\partial y_j} 
\frac{\partial y_j}{\partial z_j} 
\\
&=
\frac{\partial e}{\partial y_j} 
f'(z_j) 
\\
\frac{\partial e}{\partial w_{ij}} 
&=  
\frac{\partial e}{\partial z_j} 
\frac{\partial z_j}{\partial w_{ij}} 
\\
&= 
\frac{\partial e}{\partial z_j} \cdot x_i 
\\
\frac{\partial e}{\partial b_j} 
&=
\frac{\partial e}{\partial z_j} 
\frac{\partial z_j}{\partial b_j} 
\\
&= 
\frac{\partial e}{\partial z_j} \cdot 1 
\\
\frac{\partial e}{\partial x_i}
&=  
\sum_{j}\frac{\partial e}{\partial z_j}
\frac{\partial z_j}{\partial x_i} \\
&= 
\sum_{j}\frac{\partial e}{\partial z_j} 
\cdot w_{ij} 
\\
\end{flalign*}
$$


- vectorized version

- forward propagation @ layer $l$

$$
\begin{flalign*}
&\vec{x}=\vec{y}^{(l-1)} \\
&\vec{z}=\vec{x} @ W + \vec{b} \\
&\vec{y}= f(\vec{z}) \\
\end{flalign*}
$$


- backward propagation @ layer $l$

$$
\begin{flalign*}
&\frac{\partial e}{\partial \vec{y}}= \frac{\partial e}{\partial \vec{x}^{(l+1)}} 
\\
&\frac{\partial e}{\partial \vec{z}}=\frac{\partial e}{\partial \vec{y}} \odot f'(\vec{z}) \\ 
&\frac{\partial e}{\partial W}=\vec{x}^T @ \frac{\partial e}{\partial \vec{z}} \\
&\frac{\partial e}{\partial \vec{b}}=\frac{\partial e}{\partial \vec{z}} \\
&\frac{\partial e}{\partial \vec{x}}=\frac{\partial e}{\partial \vec{z}} @ W^T \\
\end{flalign*}
$$









